modules/CtxRefine.v
@@ -1,0 +1,215 @@
+Require Export Coqlib sflib.
+Require Import Behavior.
+Require Import Mod Skeleton.
+Require Import ModSemFacts.
+  
+Section CTX_REFINE.
+  Context `{Sk.ld}.
+  (* Contexts can be simplified as a single module (by module-linking) *)
+  Definition ctx_refines {CONF: EMSConfig} (md_tgt md_src: Mod.t): Prop :=
+    forall (ctx: Mod.t),
+      Beh.of_program (Mod.compile (Mod.add md_tgt ctx)) <1=
+      Beh.of_program (Mod.compile (Mod.add md_src ctx)).
+
+  Definition ctx_refines_strong (md_tgt md_src: Mod.t): Prop :=
+    forall (CONF: EMSConfig), ctx_refines md_tgt md_src.
+
+  Definition refines_closed {CONF: EMSConfig} (md_tgt md_src: Mod.t): Prop :=
+    Beh.of_program (Mod.compile md_tgt) <1= Beh.of_program (Mod.compile md_src).
+
+  Definition ctx_refines_list {CONF: EMSConfig} (md_tgt md_src: list Mod.t): Prop :=
+    ctx_refines (Mod.add_list md_tgt) (Mod.add_list md_src).
+
+End CTX_REFINE.
+
+Section PROPERTIES.
+  Context `{Sk.ld}.
+
+  Section CONF.
+  Context {CONF: EMSConfig}.
+
+  (*** vertical composition ***)
+  Global Program Instance refines_PreOrder: PreOrder ctx_refines.
+
+  Next Obligation. ii. ss. Qed.
+  Next Obligation. ii. eapply H1. eapply H0. ss. Qed.
+
+  Global Program Instance refines2_PreOrder: PreOrder ctx_refines_list.
+  Next Obligation.
+    ii. ss.
+  Qed.
+  Next Obligation.
+    ii. eapply H0 in PR. eapply H1 in PR. eapply PR.
+  Qed.
+
+  Global Program Instance refines_strong_PreOrder: PreOrder ctx_refines_strong.
+  Next Obligation. ii. ss. Qed.
+  Next Obligation. ii. eapply H1. eapply H0. ss. Qed.
+
+  Global Program Instance refines_closed_PreOrder: PreOrder refines_closed.
+  Next Obligation. ii; ss. Qed.
+  Next Obligation. ii; ss. eapply H1. eapply H0. eauto. Qed.
+
+  (*** horizontal composition ***)
+  Theorem refines_add
+        (md0_src md0_tgt md1_src md1_tgt: Mod.t)
+        (SIM0: ctx_refines md0_tgt md0_src)
+        (SIM1: ctx_refines md1_tgt md1_src)
+    :
+        <<SIM: ctx_refines (Mod.add md0_tgt md1_tgt) (Mod.add md0_src md1_src)>>
+  .
+  Proof. 
+    ii. r in SIM0. r in SIM1. 
+    pose proof ModFacts.add_comm as COMM. 
+    pose proof ModFacts.add_assoc as ASSOC. 
+    pose proof ModFacts.add_assoc_rev as ASSOC'. 
+    r in COMM. r in ASSOC. r in ASSOC'.
+    apply ASSOC'. 
+    apply SIM0.
+    apply ASSOC. apply COMM. apply ASSOC. apply COMM.
+    apply SIM1.
+    apply ASSOC. apply COMM. apply ASSOC.
+    apply PR.
+  Qed.
+
+  Theorem refines_proper_r
+    (mds0_src mds0_tgt: list Mod.t) (ctx: Mod.t)
+    (SIM0: ctx_refines (Mod.add_list mds0_tgt) (Mod.add_list mds0_src))
+  :
+    <<SIM: ctx_refines (Mod.add (Mod.add_list mds0_tgt) (ctx)) (Mod.add (Mod.add_list mds0_src) (ctx))>>
+  .
+  Proof.
+    ii. r in SIM0.
+    apply ModFacts.add_assoc_rev. apply ModFacts.add_assoc in PR.
+    apply SIM0. apply PR. 
+  Qed.
+
+  Theorem refines_proper_l
+    (mds0_src mds0_tgt: list Mod.t) (ctx: Mod.t)
+    (SIM0: ctx_refines (Mod.add_list mds0_tgt) (Mod.add_list mds0_src))
+  :
+    <<SIM: ctx_refines (Mod.add ctx (Mod.add_list mds0_tgt)) (Mod.add ctx (Mod.add_list mds0_src))>>
+  .
+
+  Proof.
+    ii. r in SIM0.
+    pose proof ModFacts.add_comm as COMM.
+    apply COMM. apply COMM in PR.
+    apply ModFacts.add_assoc. apply ModFacts.add_assoc_rev in PR.
+    apply COMM. apply COMM in PR.
+    apply SIM0. apply PR.  
+  Qed.
+
+  Lemma refines_close: ctx_refines <2= refines_closed.
+  Proof. 
+    ii. specialize (PR Mod.empty). ss.
+    pose proof ModFacts.add_empty_r as EMP.
+    r in EMP.
+    apply EMP with (x0 := x2) in PR.
+    2: { apply ModFacts.add_empty_rev_r. et. } 
+    apply PR.
+  Qed.
+
+  Lemma refines_empty 
+    (md: Mod.t)
+  :
+    <<SIM: ctx_refines md (Mod.add md Mod.empty)>>
+  .
+  Proof. 
+    ii. 
+    pose proof ModFacts.add_comm as COMM. 
+    pose proof ModFacts.add_assoc as ASSOC. 
+    apply COMM. apply COMM in PR. apply ModFacts.add_empty_rev_r in PR.
+    apply ASSOC. et.
+  Qed.
+
+  Lemma refines_empty_rev
+  (md: Mod.t)
+  :
+  <<SIM: ctx_refines (Mod.add md Mod.empty) md>>
+  .
+  Proof. 
+    ii. 
+    pose proof ModFacts.add_comm as COMM. 
+    pose proof ModFacts.add_assoc_rev as ASSOC'. 
+    apply COMM. apply COMM in PR. apply ASSOC' in PR. apply ModFacts.add_empty_r in PR.
+    et.
+  Qed.
+
+  (*** horizontal composition ***)
+   Theorem refines_list_add
+         (s0 s1 t0 t1: list Mod.t)
+         (SIM0: ctx_refines_list t0 s0)
+         (SIM1: ctx_refines_list t1 s1)
+     :
+       <<SIM: ctx_refines_list [Mod.add (Mod.add_list t0) (Mod.add_list t1)] [Mod.add (Mod.add_list s0) (Mod.add_list s1)]>>
+   .
+   Proof.
+    r. unfold ctx_refines_list. eapply refines_add; et.
+   Qed.
+
+
+   Corollary refines_list_pairwise
+             (mds0_src mds0_tgt: list Mod.t)
+             (FORALL: List.Forall2 (fun md_src md_tgt => ctx_refines_list [md_src] [md_tgt]) mds0_src mds0_tgt)
+     :
+       ctx_refines_list mds0_src mds0_tgt.
+   Proof.
+    induction FORALL; ss.
+    hexploit refines_list_add.
+    { eapply H0. }
+    { eapply IHFORALL. }
+    r. i.
+    induction l, l'; et.
+    { r in H1. unfold ctx_refines_list in H1. ii. apply refines_empty in PR. apply H1. unfold Mod.add_list.
+      unfold Mod.add_list in PR. apply PR. }
+    { r in H1. unfold ctx_refines_list in H1. ii. unfold Mod.add_list in H1 at 2 5 6. apply H1 in PR.
+      unfold Mod.add_list in PR. apply refines_empty_rev in PR. apply PR. }
+   Qed.
+
+   Lemma refines_list_eq (mds0 mds1: list Mod.t)
+     :
+       ctx_refines_list mds0 mds1 <-> ctx_refines (Mod.add_list mds0) (Mod.add_list mds1).
+   Proof.
+     split.
+     { ii. eapply H0. auto. }
+     { ii. eapply H0. auto. }
+   Qed.
+
+  Lemma refines_strong_refines: ctx_refines_strong <2= ctx_refines.
+  Proof. ii. eapply PR; et. Qed.
+   
+  End CONF.
+
+  Theorem refines_strong_add
+        (md0_src md0_tgt md1_src md1_tgt: Mod.t)
+        (SIM0: ctx_refines_strong md0_tgt md0_src)
+        (SIM1: ctx_refines_strong md1_tgt md1_src)
+    :
+      <<SIM: ctx_refines_strong (Mod.add md0_tgt md1_tgt) (Mod.add md0_src md1_src)>>
+  .
+  Proof.
+    intros CONF. eapply (@refines_add CONF); apply refines_strong_refines; et.
+  Qed.
+
+  Theorem refines_strong_proper_r
+        (mds0_src mds0_tgt: list Mod.t) (ctx: Mod.t)
+        (SIM0: ctx_refines_strong (Mod.add_list mds0_tgt) (Mod.add_list mds0_src))
+    :
+      <<SIM: ctx_refines_strong (Mod.add (Mod.add_list mds0_tgt) ctx) (Mod.add (Mod.add_list mds0_src) ctx)>>
+  .
+  Proof.
+    intros CONF. eapply (@refines_proper_r CONF); et.
+  Qed.
+
+  Theorem refines_strong_proper_l
+        (mds0_src mds0_tgt: list Mod.t) (ctx: Mod.t)
+        (SIM0: ctx_refines_strong (Mod.add_list mds0_tgt) (Mod.add_list mds0_src))
+    :
+      <<SIM: ctx_refines_strong (Mod.add ctx (Mod.add_list mds0_tgt)) (Mod.add ctx (Mod.add_list mds0_src))>>
+  .
+  Proof.
+    intros CONF. eapply (@refines_proper_l CONF); et.
+  Qed.
+
+End PROPERTIES.
